Pushed changes

StateSpaceTheorems.v
@@ -7,25 +7,41 @@ Require Import New.Ring.
 Require Import New.RingTheorems.
 Require Import New.Field.
 Require Import InnerProd.
+Require Import InnerProdTheorems.
 Require Import Scalars.
 Require Import States.
+Require Import StateTheorems.
 Require Import StateSpace.
+Require Import Coq.Sets.Ensembles.
 
+Variable Scalar : Type.
+Variable State : Type.
 
-Lemma state_join_bot Scalar State
+Definition equal_inner_prod_forall
+ {statespace : StateSpace Scalar State}
+ (S1 S2 : State) (S0 : State) := <| S0 | S1 |> = <| S0 | S2 |>.
+
+Definition state_join_bot
+  {statespace : StateSpace Scalar State}
+  (s : State) := join null s = s.
+
+Lemma state_join_bot_inductive
   {statespace : StateSpace Scalar State} :
-  forall (s : State), join null s = s.
+  state_pred_inductive state_join_bot.
 Proof.
+  unfold state_pred_inductive.
+  unfold state_join_bot.
+  split.
   intros.
-  apply inner_prod_ext_ind_eq.
+  apply inner_prod_ext_eq.
   intros.
-  rewrite inner_prod_join.
-  rewrite 2! inner_prod_right_strict.
-  rewrite add_zero_right.
+  rewrite inner_prod_left_join.
+  apply inner_prod_ext_eq.
+  intros.
+  rewrite inner_prod_join_right.
+  rewrite inner_prod_right_strict.
   rewrite add_zero_left.
-  rewrite <- inner_prod_join.
-  rewrite add_comm at 1.
-  intro.
+  reflexivity.
 Qed.
 
 End StateSpaceTheorems.
