StateSpace.v
@@ -10,20 +10,9 @@ Require Import InnerProd.
 Class StateSpace Scalar State := {
   scalarops_ss :> ScalarOps Scalar;
   stateops_ss :> StateOps Scalar State;
-  innerprodop_ss :> InnerProdOp Scalar State;
   innerprod_ss :> InnerProd Scalar State;
-  inner_prod_ext_ind_eq :
-    forall s1 s2 : State,
-      (forall s3 s4 : State,
-        (<| s3 | s1 |> = <| s3 | s2 |>) ->
-        (<| s4 | s1 |> = <| s4 | s2 |>) ->
-        <| join s3 s4 | s1 |> = <| join s3 s4 | s2 |>) ->
-      (forall s3 s4 : State,
-        (<| s3 | s1 |> = <| s3 | s2 |>) ->
-        (<| s4 | s1 |> = <| s4 | s2 |>) ->
-        <| meet s3 s4 | s1 |> = <| meet s3 s4 | s2 |>) ->
-      (forall s0 : State,
-        (<| s0 | s1 |> = <| s0 | s2 |>) ->
-        <| ~ s0 | s1 |> = <| ~ s0 | s2 |>) ->
-      s1 = s2
+  innerprodop_ss :> InnerProdOp Scalar State;
+  inner_prod_ext_eq :
+    forall (S1 S2 : State),
+      (forall (S0 : State), <| S0 | S1 |> = <| S0 | S2 |>) -> S1 = S2
 }.
